Fix top-level forward_simulation_same_safe_prefix

RSC_DC_MD_Instance.v
@@ -12,6 +12,8 @@ Require Import S2I.Compiler.
 Require Import S2I.Definitions.
 Require Import Definability.
 
+Set Bullet Behavior "Strict Subproofs".
+
 Module Source_Instance <: Source_Sig.
   Definition program :=
     @Source.program.
@@ -186,8 +188,32 @@ Module Compiler_Instance <: Compiler_Sig Source_Instance
   (* Definition S_simulates_I := *)
   (*   @Compiler.S_simulates_I. *)
 
-  Definition forward_simulation_same_safe_prefix :=
-    @Compiler.forward_simulation_same_safe_prefix.
+  Theorem forward_simulation_same_safe_prefix:
+    forall p p_compiled c c_compiled m,
+      linkable (Source.prog_interface p) (Source.prog_interface c) ->
+      Source.closed_program (Source.program_link p c) ->
+      Source.well_formed_program p ->
+      Source.well_formed_program c ->
+      CompCertExtensions.does_prefix (Source_Instance.CS.sem (Source.program_link p c)) m ->
+      CompCertExtensions.not_wrong_finpref m ->
+      compile_program p = Some p_compiled ->
+      compile_program c = Some c_compiled ->
+      CompCertExtensions.does_prefix (Intermediate_Instance.CS.sem (Intermediate.program_link p_compiled c_compiled)) m.
+  Proof.
+    intros p p_compiled c c_compiled m
+           Hlinkable Hclosed Hwfp Hwfc Hprefix Hnot_wrong Hcompp Hcompc.
+    pose proof Source.linking_well_formedness Hwfp Hwfc Hlinkable as Hwfpc.
+    destruct (Compiler.well_formed_compilable _ Hwfpc) as [pc_compiled Hcomppc].
+    pose proof Compiler.forward_simulation_same_safe_prefix _ _ _
+         Hclosed Hwfpc Hprefix Hnot_wrong Hcomppc
+      as [beh [Hbeh Hprefix_beh]].
+    pose proof Compiler.separate_compilation_weaker _ _ _ _ _
+         Hwfp Hwfc Hlinkable Hcompp Hcompc Hcomppc
+      as Hsc.
+    exists beh. split.
+    - apply Hsc. exact Hbeh.
+    - exact Hprefix_beh.
+  Qed.
 
   Definition backward_simulation_behavior_improves_prefix :=
     @Compiler.backward_simulation_behavior_improves_prefix.
